src/lcertify/FindCertify.v
@@ -1,0 +1,106 @@
+Require Import Relations.
+Require Import EquivDec.
+Require Import Equality.
+Require Import List.
+Require Import Bool.
+Require Import Lia.
+Require Import NArith.
+Require Import PArith.
+Require Import ZArith.
+Require Import FMapPositive.
+Require Import FSetPositive.
+Require Import EquivDec.
+Require Import sflib.
+Require Import HahnSets.
+
+Require Import PromisingArch.lib.Basic.
+Require Import PromisingArch.lib.Order.
+Require Import PromisingArch.lib.Time.
+Require Import PromisingArch.lib.Lang.
+Require Import PromisingArch.promising.Promising.
+Require Import PromisingArch.lcertify.Certify.
+Require Import PromisingArch.lcertify.CertifySim.
+
+Set Implicit Arguments.
+
+
+Inductive certified_promise (tid:Id.t) (eu1:ExecUnit.t (A:=unit)) (loc:Loc.t) (val:Val.t): Prop :=
+| certified_promise_intro
+    eu2 eu3 eu4 mem2' view_pre
+    (STEP2: rtc (certify_step tid) eu1 eu2)
+    (STEP3: write_step tid loc val view_pre eu2 eu3)
+    (STEP4: rtc (certify_step tid) eu3 eu4)
+    (MEM: eu2.(ExecUnit.mem) = eu1.(ExecUnit.mem) ++ mem2')
+    (MEM2': Forall (fun msg => msg.(Msg.loc) <> loc) mem2')
+    (VIEW_PRE: view_pre.(View.ts) <= length eu1.(ExecUnit.mem))
+.
+
+Theorem certified_promise_complete
+        tid (eu1 eu2:ExecUnit.t (A:=unit)) loc val ts
+        (STATE: eu1.(ExecUnit.state) = eu2.(ExecUnit.state))
+        (LOCAL: Local.promise loc val ts tid
+                              eu1.(ExecUnit.local) eu1.(ExecUnit.mem)
+                              eu2.(ExecUnit.local) eu2.(ExecUnit.mem))
+        (CERTIFY: certify tid eu2):
+  certified_promise tid eu1 loc val.
+Proof.
+Admitted.
+
+Lemma promise_sim_eu
+      tid (eu1:ExecUnit.t (A:=unit)) loc val
+      (WF: ExecUnit.wf tid eu1):
+  exists eu2,
+    <<STEP: Local.promise loc val (S (length eu1.(ExecUnit.mem))) tid
+                          eu1.(ExecUnit.local) eu1.(ExecUnit.mem)
+                          eu2.(ExecUnit.local) eu2.(ExecUnit.mem)>> /\
+    <<SIM: sim_eu tid (length eu1.(ExecUnit.mem)) (Promises.set (S (length eu1.(ExecUnit.mem))) bot) eu2 eu1>>.
+Proof.
+  destruct eu1 as [st1 lc1 mem1]. eexists (ExecUnit.mk st1 _ _). splits; ss.
+  econs; ss.
+  - admit. (* sim_state refl *)
+  - econs; ss.
+    + admit. (* sim_fwdbank *)
+    + admit. (* sim_exbank *)
+    + i. rewrite Promises.set_o. condtac; ss. clear X. inv e. lia.
+    + i. rewrite ? Promises.set_o, Promises.lookup_bot. condtac; ss.
+      eapply Local_wf_promises_above; eauto. apply WF.
+  - econs; ss.
+    + rewrite app_nil_r. ss.
+    + i. revert TSP. rewrite Promises.set_o, Promises.lookup_bot. condtac; ss. clear X. inv e.
+      rewrite app_length. s. clear. lia.
+    + i. revert TSP. rewrite Promises.set_o, Promises.lookup_bot. condtac; ss. clear X. inv e.
+      apply nth_error_snoc_inv in MSG. des; subst; ss.
+      * lia.
+      * splits; ss. inv WF. inv LOCAL. ss. eapply le_lt_trans; [apply COH|]. ss.
+    + i. apply nth_error_singleton_inv in NTH. des. subst.
+      revert PROMISES. rewrite Promises.set_o. condtac; ss.
+      exfalso. apply c. rewrite Time.add_0_r. refl.
+Admitted.
+
+Theorem certified_promise_sound
+        tid (eu1:ExecUnit.t (A:=unit)) loc val
+        (WF: ExecUnit.wf tid eu1)
+        (CERTIFY: certified_promise tid eu1 loc val):
+  exists eu2 ts,
+    <<STATE: eu1.(ExecUnit.state) = eu2.(ExecUnit.state)>> /\
+    <<LOCAL: Local.promise loc val ts tid
+                           eu1.(ExecUnit.local) eu1.(ExecUnit.mem)
+                           eu2.(ExecUnit.local) eu2.(ExecUnit.mem)>> /\
+    <<CERTIFY: certify tid eu2>>.
+Proof.
+  inv CERTIFY.
+  exploit promise_sim_eu; eauto. i. des. rename eu0 into eu1', STEP into STEP1', SIM into SIM1.
+  exploit sim_eu_rtc_step; eauto.
+  { i. revert TSP. rewrite Promises.set_o. condtac; ss. clear X. inv e.
+    admit. (* view_pre *)
+  }
+  { admit. (* wf *) }
+  { rewrite <- VIEW_PRE.
+    destruct eu2 as [st2 lc2 mem2].
+    destruct eu3 as [st3 lc3 mem3].
+    inv STEP3. inv PROMISE. inv FULFILL. inv WRITABLE. ss. subst.
+    rewrite <- join_r, <- join_r, <- join_l. ss.
+  }
+  i. des. rename eu1'0 into eu2', STEP into STEP2', SIM into SIM2.
+  admit. (* [write] and [to-the-end] *)
+Admitted.
